Verified seq

src/Compiler/CompilerCorrectness.v
@@ -1,33 +1,262 @@
-From Coq         Require Import String ZArith.
+From Coq         Require Import String ZArith Morphisms List.
 From ASL         Require Import Semantics AST Theory.
-From ASLCompiler Require Import Compiler Renv.
-From Vellvm      Require Import Semantics. 
+From ASLCompiler Require Import Compiler Renv KTreeFin Fin.
+From Vellvm      Require Import Semantics Syntax. 
 From ITree       Require Import ITree ITreeFacts. 
 From LLVMExtra   Require Import Utils.
 
 Import SemNotations.
 Import ITreeNotations.
+Import ListNotations.
 
 Open Scope string_scope.
+Open Scope itree_scope.
+Open Scope list_scope.
 
-Definition eutt_inv (r1 : (env * unit)) (r2 : memory_stack * (local_env * (global_env * uvalue))) : Prop :=
-let asl_env := fst r1 in
-let m_llvm := fst r2 in
-let l_llvm := fst (snd r2) in
-let g_llvm := fst (snd (snd r2)) in
-  Renvh asl_env g_llvm l_llvm m_llvm.
+Section RAB.
 
-Definition bisimilar (t1 : itree (State +' CallE +' PickE +' UBE +' DebugE +' FailureE) unit) (t2 : itree (instr_E) uvalue)  :=
-  forall g_llvm l_llvm m_llvm g_asl,
-    Renvh g_asl g_llvm l_llvm m_llvm ->
-      eutt eutt_inv
-       (interp_asl t1 g_asl)
-       (ℑ3 t2 g_llvm l_llvm m_llvm).
+  Context {A B : Type}.
+  Context (RAB : A -> B -> Prop).
+
+  
+  Definition eutt_inv (r1 : (env * A)) (r2 : memory_stack * (local_env * (global_env * B))) : Prop :=
+  let asl_env := fst r1 in
+  let m_llvm := fst r2 in
+  let l_llvm := fst (snd r2) in
+  let g_llvm := fst (snd (snd r2)) in
+    Renvh asl_env g_llvm l_llvm m_llvm /\ RAB (snd r1) (snd (snd (snd r2))).
+
+
+  Definition bisimilar (t1 : itree (State +' CallE +' PickE +' UBE +' DebugE +' FailureE) A) (t2 : itree (instr_E) B)  :=
+    forall g_llvm l_llvm m_llvm g_asl,
+      Renvh g_asl g_llvm l_llvm m_llvm ->
+        eutt eutt_inv
+         (interp_asl t1 g_asl)
+         (ℑ3 t2 g_llvm l_llvm m_llvm).
+
+End RAB.
+
+
+Global Instance eutt_bisimilar {A B}  (RAB : A -> B -> Prop):
+    Proper (eutt eq ==> eutt eq ==> iff) (@bisimilar A B RAB).
+  Proof.
+    repeat intro.
+    unfold bisimilar. split.
+    - intros.
+      rewrite <- H, <- H0. auto.
+    - intros.
+      rewrite H, H0. auto.
+  Qed.
+
+
+ Definition to_itree' {E A} (f : ktree_fin E 1%nat A) : itree E (fin A) := f f0.
+  Lemma fold_to_itree' {E} (f : ktree_fin E 1%nat 1%nat) : f f0 = to_itree' f.
+  Proof. reflexivity. Qed.
+
+  Global Instance Proper_to_itree' {E A} :
+    Proper (eq2 ==> eutt eq) (@to_itree' E A).
+  Proof.
+    repeat intro.
+    apply H.
+  Qed.
+
+
+Check bisimilar.
+
+ Lemma bisimilar_bind' {A A' B C}  (RAA' : A -> A' -> Prop) (RBC: B -> C -> Prop):
+    forall (t1 : itree (State +' CallE +' PickE +' UBE +' DebugE +' FailureE) A) (t2 : itree (instr_E) A') ,
+      bisimilar RAA' t1 t2 ->
+      forall (k1 : A -> itree (State +' CallE +' PickE +' UBE +' DebugE +' FailureE) B) (k2 : A' -> itree (instr_E) C)
+        (H: forall (a:A) (a':A'), bisimilar RBC (k1 a) (k2 a')),
+        bisimilar RBC (t1 >>= k1) (t2 >>= k2).
+  Proof.
+    repeat intro.
+    rewrite InterpreterCFG.interp_cfg3_bind .
+    rewrite interp_imp_bind.
+    eapply eutt_clo_bind.
+    { eapply H; auto. }
+    intros.
+    destruct u1 as [? ?].
+    destruct u2 as [? [? [? ?]]].
+    unfold eutt_inv in H2.
+    simpl in H2. destruct H2. subst.
+    eapply H0; eauto.
+  Qed.
+
+
+
+Definition TT {A B}: A -> B -> Prop  := fun _ _ => True.
+Hint Unfold TT: core.
+
+
+Lemma ignore_ret_r : forall A (t1 : itree (State +' CallE +' PickE +' UBE +' DebugE +' FailureE) unit) (t2 : itree (instr_E) A) (u : uvalue), 
+  bisimilar TT t1 t2 -> bisimilar TT t1 (t2;; Ret u).
+Proof.
+
+  intros.
+  rewrite <- (bind_ret_r t1) at 1.
+  apply bisimilar_bind' with (RAA':=TT); auto.
+  intros.
+  unfold bisimilar.
+  intros.
+  rewrite interp_asl_ret.
+  rewrite InterpreterCFG.interp_cfg3_ret.
+  apply eqit_Ret.
+  red; simpl.
+  auto.
+Qed.
+
+Lemma ignore_ret_l : forall A (t1 : itree (State +' CallE +' PickE +' UBE +' DebugE +' FailureE) unit) (t2 : itree (instr_E) A), 
+  bisimilar TT t1 t2 -> bisimilar TT (t1 ;; Ret tt) t2.
+Proof.
+
+  intros.
+  rewrite <- (bind_ret_r t2) at 1.
+  apply bisimilar_bind' with (RAA':=TT); auto.
+  intros.
+  unfold bisimilar.
+  intros.
+  rewrite interp_asl_ret.
+  rewrite InterpreterCFG.interp_cfg3_ret.
+  apply eqit_Ret.
+  red; simpl.
+  auto.
+Qed.
+ 
+
+Lemma bisimilar_bind_ret : forall A (t1 : itree (State +' CallE +' PickE +' UBE +' DebugE +' FailureE) unit) (t2 : itree (instr_E) A), 
+bisimilar TT (t1;; Ret tt) t2 ->
+bisimilar TT t1 t2.
+Proof.
+  intros.
+  unfold bisimilar.
+  setoid_rewrite interp_asl_bind_ret.
+  assumption.
+Qed.
 
 
 Theorem compiler_correct (s:stmt) :
-  bisimilar (denote_asl s) (denote_cfg (compile s)).
+  bisimilar TT (denote_asl s) (denote_code (compile s)).
 Proof.
+
+  induction s.
+  + simpl.
+    (* Because our expressions can only be Lit, destruct will only throw one case *)
+    destruct e; simpl.
+    setoid_rewrite DenotationTheory.denote_code_singleton.
+    unfold gen_alloc_instr.    
+    rewrite InterpreterCFG.interp_cfg3_bind.
+    rewrite simpl_alloca_assign.
+    repeat rewrite bind_ret_.  
+    rewrite InterpreterCFG.interp_cfg3_ret.
+    rewrite interp_asl_SetVar.
+    red.
+    apply eqit_Ret.
+    unfold eutt_inv. simpl.
+    split.
+    - apply RenvhAssign. auto.
+    - auto.
+  + simpl. 
+    unfold generate_cfg.
+    rewrite DenotationTheory.denote_code_app_eq_itree.
+    apply bisimilar_bind' with (RAA' := TT).
+    - assumption.
+    - intros. assumption.
+  + simpl.
+    rewrite DenotationTheory.denote_code_nil.
+    unfold bisimilar.
+    intros.
+    rewrite interp_asl_ret.
+    rewrite InterpreterCFG.interp_cfg3_ret.
+    apply eqit_Ret.
+    unfold eutt_inv.
+    auto.
+
+
+
+ (*    simpl.
+
+  setoid_rewrite simpl_block.
+ rewrite bind_bind.
+  setoid_rewrite bind_ret_. 
+  rewrite DenotationTheory.denote_code_app_eq_itree.
+  
+  apply bisimilar_bind_ret.
+  apply bisimilar_bind' with (RAA' := TT) .
+  - unfold bisimilar.
+    apply bisimilar_bind' with (RAA' := TT) .
+    --  unfold denote_cfg in IHs1.
+        unfold generate_cfg in IHs1.
+        simpl in IHs1.
+        rewrite simpl_block in IHs1.
+        rewrite bind_bind in IHs1.
+        setoid_rewrite bind_ret_ in IHs1. 
+        unfold bisimilar in IHs1.
+        unfold bisimilar.
+        intros.
+        rewrite interp_cfg3_bind_ret.
+        apply IHs1 in H.
+        give_up.
+    rewrite interp_cfg3_bind_ret.
+  - 
+  
+ *)
+ 
+  unfold bisimilar.
+  rewrite interp_asl_bind_ret.
+
+  rewrite <- ignore_ret_l.
+  apply bisimilar_bind' with (RAA' := TT) .
+
+  assert (bisimilar TT (denote_asl s1;; denote_asl s2) ((⟦ gen_body_code s1 ⟧c;; ⟦ gen_body_code s2 ⟧c))).
+  {
+  apply bisimilar_bind' with (RAA' := TT) .
+  + 
+    unfold denote_cfg in IHs1.
+    unfold generate_cfg in IHs1.
+    simpl in IHs1.
+    rewrite simpl_block in IHs1.
+    rewrite bind_bind in IHs1.
+    setoid_rewrite bind_ret_ in IHs1. 
+    apply ignore_ret_l in IHs1; auto.
+    give_up.
+  +
+  intros.
+  unfold denote_cfg in IHs2.
+    unfold generate_cfg in IHs2.
+    simpl in IHs2.
+    rewrite simpl_block in IHs2.
+    rewrite bind_bind in IHs2.
+    setoid_rewrite bind_ret_ in IHs2. 
+
+  }
+
+  apply bisimilar_bind' with (RAA' := TT).
+  - apply bisimilar_bind' with (RAA' := TT).
+  
+
+  assert (bisimilar TT (denote_asl s1;; denote_asl s2) ((⟦ nil ⟧c;; Ret (UVALUE_I32 (Int32.repr 1))))). {
+  
+    rewrite DenotationTheory.denote_code_nil.
+    apply bisimilar_bind' with (RAA' := TT).
+    + unfold bisimilar.
+      intros.
+
+    rewrite DenotationTheory.denote_code_app_eq_itree .
+
+
+    eapply bisimilar_bind'.
+
+  }
+
+  eapply bisimilar_ret'.
+
+
+
+  eapply bisimilar_bind'.
+
+  unfold denote_asl; simpl.
+
   unfold bisimilar.
   intros.
   unfold denote_cfg; simpl.
@@ -38,6 +267,7 @@ Proof.
   induction s.
   
   + (* Assign *) 
+    
     rewrite DenotationTheory.denote_code_app.
     simpl.
     (* Because our expressions can only be Lit, destruct will only throw one case *)
@@ -51,10 +281,16 @@ Proof.
     rewrite interp_asl_SetVar.
     red.
     apply eqit_Ret.
-
     unfold eutt_inv. simpl.
-    apply RenvhAssign.
-    auto.
+    split.
+    - apply RenvhAssign. auto.
+    - auto.
+  + (* Seq *)
+    simpl.
+    apply bisimilar_bind' with (RAA' := TT) (RBC := TT) .
+    apply bisimilar_bind' RAA', RBC, t1, t2, k1, k2. in H.
+
+
   + (* Skip *)
     rewrite DenotationTheory.denote_code_nil.
     repeat rewrite bind_ret_.
@@ -62,5 +298,6 @@ Proof.
     rewrite interp_asl_ret.
     red.
     apply eqit_Ret.
+    unfold eutt_inv.
     auto.
 Qed.
